finish hw6

lean/LoVe/LoVe06_InductivePredicates_HomeworkSheet.lean
@@ -27,22 +27,27 @@ inductive Term : Type
 /- 1.1 (2 points). Define an inductive predicate `IsLam` that returns `True` if
 its argument is of the form `Term.lam …` and that returns `False` otherwise. -/
 
+inductive IsLam : Term → Prop
+  | lam : IsLam (Term.lam _ _)
+
 -- enter your definition here
 
 /- 1.2 (2 points). Validate your answer to question 1.1 by proving the following
 theorems: -/
 
 theorem IsLam_lam (s : String) (t : Term) :
-    IsLam (Term.lam s t) :=
-  sorry
+    IsLam (Term.lam s t) := by
+  exact IsLam.lam
 
 theorem not_IsLamVar (s : String) :
-    ¬ IsLam (Term.var s) :=
-  sorry
+    ¬ IsLam (Term.var s) := by
+    intro isLam
+    cases isLam
 
 theorem not_IsLam_app (t u : Term) :
-    ¬ IsLam (Term.app t u) :=
-  sorry
+    ¬ IsLam (Term.app t u) := by
+    intro isLam
+    cases isLam
 
 
 /- ## Question 2 (6 points): Transitive Closure
@@ -69,6 +74,9 @@ would use replace `(step)` with the following right-leaning rule:
 Define a predicate `TCV2` that embodies this alternative definition. -/
 
 -- enter your definition here
+inductive TCV2 {α : Type} (R : α → α → Prop) : α → α → Prop
+  | base (a b : α)   : R a b → TCV2 R a b
+  | pets (a b c : α) : TCV2 R a b → R b c → TCV2 R a c
 
 /- 2.2 (2 points). Yet another definition of the transitive closure `R⁺` would
 use the following symmetric rule instead of `(step)` or `(pets)`:
@@ -76,6 +84,9 @@ use the following symmetric rule instead of `(step)` or `(pets)`:
     (trans) for all `a, b, c ∈ A`, if `a R⁺ b` and `b R⁺ c`, then `a R⁺ c`.
 
 Define a predicate `TCV3` that embodies this alternative definition. -/
+inductive TCV3 {α : Type} (R : α → α → Prop) : α → α → Prop
+  | base (a b : α)   : R a b → TCV3 R a b
+  | trans (a b c : α) : TCV3 R a b → TCV3 R b c → TCV3 R a c
 
 -- enter your definition here
 
@@ -83,13 +94,26 @@ Define a predicate `TCV3` that embodies this alternative definition. -/
 
 theorem TCV3_step {α : Type} (R : α → α → Prop) (a b c : α) (rab : R a b)
       (tbc : TCV3 R b c) :
-    TCV3 R a c :=
-  sorry
+    TCV3 R a c := by
+  have tab: TCV3 R a b := TCV3.base a b rab
+  apply TCV3.trans a b
+  · exact tab
+  · exact tbc
+
 
 /- 2.4 (1 point). Prove the following theorem by rule induction: -/
 
 theorem TCV1_pets {α : Type} (R : α → α → Prop) (c : α) :
-    ∀a b, TCV1 R a b → R b c → TCV1 R a c :=
-  sorry
-
+    ∀a b, TCV1 R a b → R b c → TCV1 R a c := by
+  intro a b
+  intro tab rbc
+  induction tab with
+  | base a b ih =>
+    apply TCV1.step a b c
+    · apply ih
+    · apply TCV1.base b c rbc
+  | step a b' b ih ih2 ih3 =>
+    have tb'c : TCV1 R b' c := ih3 rbc
+    have tac : TCV1 R a c := by apply TCV1.step a b' c ih tb'c
+    exact tac
 end LoVe
